\documentclass{article}
\usepackage[top=1in, bottom=1in, left=1in, right=1in]{geometry}
\usepackage{amsmath}
\begin{document}

\begin{flushright}
Matt Jibson \\
ST 521 \\
HW 2
\end{flushright}

\begin{enumerate}
\item %1
	\begin{enumerate}
		\item Markov chain - state space is $\{0, 1, 2, 3, 4, 5, 6\}$.
			\begin{displaymath}
				P = \left( \begin{array}{ccccccc}
					0 & 1/6 & 1/6 & 1/6 & 1/6 & 1/6 & 1/6 \\
					0 & 1/6 & 1/6 & 1/6 & 1/6 & 1/6 & 1/6 \\
					0 & 0 & 2/6 & 1/6 & 1/6 & 1/6 & 1/6 \\
					0 & 0 & 0 & 3/6 & 1/6 & 1/6 & 1/6 \\
					0 & 0 & 0 & 0 & 4/6 & 1/6 & 1/6 \\
					0 & 0 & 0 & 0 & 0 & 5/6 & 1/6 \\
					0 & 0 & 0 & 0 & 0 & 0 & 1
				\end{array} \right)
			\end{displaymath}
		\item Markov chain - state space is $\{0, 1, 2, \dots\}$.
			\begin{displaymath}
				P = \left( \begin{array}{ccccc}
					5/6 & 1/6 & 0 & \cdots \\
					0 & 5/6 & 1/6 & 0 & \cdots \\
					\vdots & \ddots & \ddots & \ddots & \ddots
				\end{array} \right)
			\end{displaymath}
		\item Not Markov chain since current state depends on its distance from the previous six.
		\item Markov chain - state space is $\{0, 1, 2, \dots\}$.
			\begin{displaymath}
				P = \left( \begin{array}{ccccc}
					\frac{1}{6} & \frac{1}{6} (\frac{5}{6})^1 & \frac{1}{6} (\frac{5}{6})^2 & \dots \\
					0 & \frac{1}{6} & \frac{1}{6} (\frac{5}{6})^1 & \frac{1}{6} (\frac{5}{6})^2 & \dots \\
					\vdots & \ddots & \ddots & \ddots & \ddots
				\end{array} \right)
			\end{displaymath}
	\end{enumerate}
\item %2
	\begin{displaymath}
		P = \left( \begin{array}{cccc}
			.1 & .3 & .2 & .4 \\
			0 & .4 & .2 & .4 \\
			0 & 0 & .6 & .4 \\
			0 & 0 & 0 & 1
		\end{array} \right)
	\end{displaymath}
\item %3
	\begin{displaymath}
		P^3 = \left( \begin{array}{ccc}
			.478 & .264 & .258 \\
			.36 & .256 & .384 \\
			.57 & .18 & .25
		\end{array} \right),
		P^4 = \left( \begin{array}{ccc}
			.4636 & .254 & .2824 \\
			.444 & .2256 & .3304 \\
			.524 & .222 & .254
		\end{array} \right)
	\end{displaymath}
	$P(\{X_3 = 1 | X_0 = 0\}) = 0.264$ \\
	$P(\{X_4 = 1 | X_0 = 0\}) = 0.254$
\item %4
	$P(Y_n = s | Y_{n-1} = y_{n-1}) = P(h(X_n) = s | h(X_{n-1}) = h(x_{n-1}))$. \\
	This does not necessarily work if $h$ is not one-to-one.
\item %5
	\begin{enumerate}
		\item Markov chain.
		\item Not Markov chain.
	\end{enumerate}
\item %6
\end{enumerate}

\end{document}